lean4/Automaton/Regex/Basic.lean
@@ -1,11 +1,10 @@
 import Automaton.Language.Basic
 import Mathlib.Data.Finset.Basic
 import Mathlib.Data.Fin.Basic
-import Automaton.NFA.ENFA
 
 namespace Regex
 
-open Set Finset εNFA
+open Set Finset
 
 inductive Regex (f : Finset α) : Type u
   | zero : Regex f
@@ -19,9 +18,13 @@ open Regex
 
 variable {α : Type _} [DecidableEq α] (f : Finset α)
 
-inductive starLang (l : Lang f) : Lang f where
-  | empty : starLang l []
-  | star  : ∀ u w : List f, u ∈ l → w ∈ l → starLang l (u++w)
+inductive plusLang (P : Lang α) : Lang α where
+| empty :  ∀ w ∈ P, plusLang P w
+| extend : ∀ u w, P u → plusLang P w → plusLang P (u ++ w)
+
+inductive starLang (P : Lang α) : Lang α where
+| empty : starLang P []
+| extend : ∀ u w, P u → starLang P w → starLang P (u ++ w)
 
 def RegexLan : Regex f → Lang f
   | zero => ∅
@@ -29,47 +32,45 @@ def RegexLan : Regex f → Lang f
   | char a => {[a]}
   | plus a b => RegexLan a ∪ RegexLan b
   | append a b => {w | ∃ x y, x ∈ RegexLan a ∧ y ∈ RegexLan b ∧ w = x++y}
-  | star a => starLang f (RegexLan a)
+  | star a => starLang (RegexLan a)
 
 
-def ZeroεNFA : εNFA f {0} := {q₀ := {⟨0,by simp⟩} , fs := {} , δ := fun _ _ => {⟨0,by simp⟩}}
-def EpsilonεNFA : εNFA f {0} := {q₀ := {⟨0,by simp⟩} , fs := {⟨0,by simp⟩} , δ := fun _ _ => ∅}
-def CharεNFA (c : f) : εNFA f {0,1} := {q₀ := {⟨0,by simp⟩} , fs := {⟨1,by simp⟩} , δ := fun q e => if q = ⟨0,by simp⟩ ∧ e = c then {⟨1,by simp⟩} else ∅}
+-- def ZeroεNFA : εNFA f {0} := {q₀ := {⟨0,by simp⟩} , fs := {} , δ := fun _ _ => {⟨0,by simp⟩}}
+-- def EpsilonεNFA : εNFA f {0} := {q₀ := {⟨0,by simp⟩} , fs := {⟨0,by simp⟩} , δ := fun _ _ => ∅}
+-- def CharεNFA (c : f) : εNFA f {0,1} := {q₀ := {⟨0,by simp⟩} , fs := {⟨1,by simp⟩} , δ := fun q e => if q = ⟨0,by simp⟩ ∧ e = c then {⟨1,by simp⟩} else ∅}
 
 
-lemma ZeroεNFALang : εNFA_lang (ZeroεNFA f) = ∅ := by
-  simp only [εNFA_lang,εnfa_accepts,ZeroεNFA,Finset.inter_empty]
-  trivial
+-- lemma ZeroεNFALang : εNFA_lang (ZeroεNFA f) = ∅ := by
+--   simp only [εNFA_lang,εnfa_accepts,ZeroεNFA,Finset.inter_empty]
+--   trivial
 
 
-lemma EpsilonεNFAW : δ_star (EpsilonεNFA f) w = ∅ := by
-  induction w using List.reverseRecOn with
-  | H0 => sorry
-  | H1 e es s => simp [δ_star,δ_star']
+-- lemma EpsilonεNFAW : δ_star (EpsilonεNFA f) w = ∅ := by
+--   induction w using List.reverseRecOn with
+--   | H0 => sorry
+--   | H1 e es s => simp [δ_star,δ_star']
+--                  sorry
 
-lemma EpsilonεNFALang : εnfa_accepts (EpsilonεNFA f) w ↔ w = [] := by
-  apply Iff.intro
-  · intro ac
-    simp only [εnfa_accepts,EpsilonεNFA] at ac
-    match w with
-    | [] => simp
-    | e::es => induction es with
-               | nil => simp [Finset.Nonempty,δ_star,δ_star',Finset.biUnion] at ac
-                        rw [εclosure_eq_εclosure] at ac
-                        split at ac
-                        · trivial
-                        · trivial
-               | cons e es s => simp at s
-                                simp only [δ_star] at ac
-
-
-
-  · intro w
-    rw [w]
-    simp [εnfa_accepts,δ_star,δ_star',EpsilonεNFA,Finset.Nonempty]
-    apply εclosure_start_mem
-    simp
-
+-- lemma EpsilonεNFALang : εnfa_accepts (EpsilonεNFA f) w ↔ w = [] := by
+--   apply Iff.intro
+--   · intro ac
+--     simp only [εnfa_accepts,EpsilonεNFA] at ac
+--     match w with
+--     | [] => simp
+--     | e::es => induction es with
+--                | nil => simp [Finset.Nonempty,δ_star,δ_star',Finset.biUnion] at ac
+--                         rw [εclosure_eq_εclosure] at ac
+--                         split at ac
+--                         · trivial
+--                         · trivial
+--                | cons e es s => simp at s
+--                                 simp only [δ_star] at ac
+--                                 sorry
+--   · intro w
+--     rw [w]
+--     simp [εnfa_accepts,δ_star,δ_star',EpsilonεNFA,Finset.Nonempty]
+--     apply εclosure_start_mem
+--     simp
 
 
 
