lean4/Automaton/Regex/ToNFA.lean
@@ -1,0 +1,502 @@
+import Automaton.NFA.Basic
+import Automaton.NFA.ToDFA
+import Automaton.Regex.Basic
+import Automaton.DFA.Basic
+import Automaton.Language.Basic
+
+open NFA ToDFA
+
+variable {σ : Type _} {q : Type _} {σs : Finset σ} {qs : Finset q} (t : NFA σs qs) [DecidableEq σ] [DecidableEq q]
+
+
+def starNFA_δ : qs → σs → Finset qs := fun q σ => if Finset.Nonempty (t.δ q σ ∩ t.fs) then t.δ q σ ∪ t.q₀ else t.δ q σ
+
+def starNFA : NFA σs qs := {q₀ := t.q₀, fs := t.fs, δ := starNFA_δ t}
+
+theorem δ_star'_union_char (q : Finset qs) : Finset.Nonempty (δ_step t q e ∩ t.fs) → δ_star' (starNFA t) q [e] = δ_star' t q [e] ∪ t.q₀ := by
+  intro h
+  simp only [δ_star,δ_star',δ_step]
+  simp only [δ_step] at h
+  simp only [starNFA,starNFA_δ]
+  apply Finset.eq_iff_fa_mem.mpr
+  intro q
+  apply Iff.intro
+  · intro h'
+    rw [Finset.mem_biUnion] at h'
+    rw [Finset.mem_union,Finset.mem_biUnion]
+    apply Exists.elim h'
+    intro x xin
+    split at xin
+    · rw [Finset.mem_union] at xin
+      apply Or.elim xin.2
+      · intro qin
+        apply Or.inl
+        exists x
+        exact ⟨xin.1,qin⟩
+      · intro qin
+        apply Or.inr
+        exact qin
+    · apply Or.inl
+      exists x
+  · intro h'
+    rw [Finset.mem_union,Finset.mem_biUnion] at h'
+    rw [Finset.mem_biUnion]
+    apply Or.elim h'
+    · intro ex
+      apply Exists.elim ex
+      intro x xin
+      exists x
+      split
+      · exact ⟨xin.1, Finset.mem_union_left _ xin.2⟩
+      · exact xin
+    · intro qin
+      simp only [Finset.Nonempty] at h
+      apply Exists.elim h
+      intro a ain
+      rw [Finset.mem_inter,Finset.mem_biUnion] at ain
+      apply Exists.elim ain.1
+      intro b bin
+      exists b
+      split
+      · exact ⟨bin.1, Finset.mem_union_right _ qin⟩
+      · have : False := by have : ¬Finset.Nonempty (NFA.δ t b e ∩ t.fs) := by assumption
+                           apply this
+                           rw [Finset.Nonempty]
+                           exists a
+                           apply Finset.mem_inter.mpr
+                           exact ⟨bin.2, ain.2⟩
+        contradiction
+
+theorem δ_star'_union_prefinal : (q : Finset qs) → (e : σs) → Finset.Nonempty (δ_step t q e ∩ t.fs) → δ_star' (starNFA t) q (e::w) = δ_star' (starNFA t) (δ_star' t q [e] ∪ t.q₀) w := by
+  induction w using List.reverseRecOn with
+  | H0 => intro q e ne
+          simp
+          apply δ_star'_union_char
+          exact ne
+  | H1 es e s => intro q e' ne
+                 rw [←List.cons_append,←δ_star'_append_eq,s,←δ_star'_append_eq]
+                 exact ne
+
+
+theorem δ_subset_starNFA : t.δ s e ⊆ (starNFA t).δ s e := by
+  simp only [starNFA,starNFA_δ]
+  split
+  · apply Finset.subset_union_left
+  · rfl
+
+theorem δ_star'_subset_starNFA : δ_star' t s w ⊆ δ_star' (starNFA t) s w  := by
+  induction w using List.reverseRecOn with
+  | H0 => simp
+  | H1 w e ss => rw [←δ_star'_append_eq,←δ_star'_append_eq]
+                 simp only [δ_star',δ_star',δ_step,Finset.biUnion_subset]
+                 intro x xin
+                 have h : (starNFA t).δ x e ⊆ Finset.biUnion (δ_star' (starNFA t) s w) fun n => NFA.δ (starNFA t) n e := by
+                  apply Finset.subset_biUnion_of_mem (fun n => NFA.δ (starNFA t) n e)
+                  apply Finset.mem_of_subset
+                  apply ss
+                  exact xin
+                 apply Finset.instIsTransFinsetSubsetInstHasSubsetFinset.trans
+                 have : t.δ x e ⊆ (starNFA t).δ x e := by apply δ_subset_starNFA
+                 apply this
+                 exact h
+
+theorem nfa_accepts_starNFA : nfa_accepts t w → nfa_accepts (starNFA t) w := by
+  intro h
+  simp only [nfa_accepts] at h
+  simp only [nfa_accepts,Finset.Nonempty]
+  apply Finset.not_disjoint_iff_nonempty_inter.mp
+  intro h'
+  simp only [Disjoint] at h'
+  simp only [Finset.Nonempty] at h
+  apply Exists.elim h
+  intro a ain
+  have ain := Finset.mem_inter.mp ain
+  have : {a} ⊆ δ_star' (starNFA t) (starNFA t).q₀ w := by apply Finset.instIsTransFinsetSubsetInstHasSubsetFinset.trans
+                                                          have : {a} ⊆ δ_star' t t.q₀ w := by apply Finset.singleton_subset_iff.mpr
+                                                                                              exact ain.1
+                                                          apply this
+                                                          apply δ_star'_subset_starNFA
+  have := h' this
+  simp [starNFA] at this
+  apply this
+  exact ain.2
+
+
+theorem subset_δ_star'_subset : (s₁ s₂ : Finset qs) → s₁ ⊆ s₂ → δ_star' t s₁ w ⊆ δ_star' t s₂ w := by
+  induction w using List.reverseRecOn with
+  | H0 => simp [δ_star']
+  | H1 w e s => intro s₁ s₂ ss
+                rw [←δ_star'_append_eq,←δ_star'_append_eq]
+                have : δ_star' t s₁ w ⊆ δ_star' t s₂ w := by apply s; exact ss
+                simp only [δ_star',δ_step,Finset.biUnion_subset]
+                intro x xin
+                apply Finset.subset_biUnion_of_mem (fun n => NFA.δ t n e)
+                apply Finset.mem_of_subset
+                apply this
+                exact xin
+
+
+theorem starNFA_δ_inter_Nonempty_iff : Finset.Nonempty ((starNFA t).fs ∩ (starNFA t).δ a e) ↔ Finset.Nonempty (t.fs ∩ t.δ a e) := by
+  apply Iff.intro
+  · intro h
+    simp only [starNFA,starNFA_δ] at h
+    split at h
+    · rwa [Finset.inter_comm]
+    · exact h
+  · intro h
+    simp only [starNFA,starNFA_δ]
+    split
+    · simp only [Finset.Nonempty]
+      simp only [Finset.Nonempty] at h
+      apply Exists.elim h
+      intro q qin
+      exists q
+      apply Finset.mem_inter.mpr
+      have := Finset.mem_inter.mp qin
+      apply And.intro
+      · exact this.1
+      · apply Finset.mem_union_left
+        exact this.2
+    · rw [Finset.inter_comm] at h
+      contradiction
+
+
+theorem starNFA_accepts_start_subset : nfa_accepts (starNFA t) w → (starNFA t).q₀ ⊆ δ_star (starNFA t) w := by
+  intro h
+  cases List.eq_nil_or_concat w with
+  | inl g => rw [g]
+             simp [starNFA]
+  | inr g => apply Exists.elim g
+             intro l ex
+             apply Exists.elim ex
+             intro a eq
+             rw [eq] at h
+             rw [eq]
+             rw [δ_star,←δ_star'_append_eq]
+             simp only [δ_star',δ_step,starNFA]
+             simp only [nfa_accepts,δ_star,←δ_star'_append_eq,δ_star',δ_step] at h
+             rw [Finset.inter_comm,Finset.inter_biUnion] at h
+             simp only [Finset.Nonempty] at h
+             apply Exists.elim h
+             intro q qin
+             simp only [Finset.mem_biUnion] at qin
+             apply Exists.elim qin
+             intro q' qin'
+             have  := Finset.subset_biUnion_of_mem (fun n => NFA.δ (starNFA t) n a) qin'.1
+             simp only [starNFA] at this
+             have ne : Finset.Nonempty ((starNFA t).fs ∩ (starNFA t).δ q' a) := by simp only [Finset.Nonempty]
+                                                                                   exists q
+                                                                                   exact qin'.2
+             have ne' : Finset.Nonempty (t.fs ∩ NFA.δ t q' a) := (starNFA_δ_inter_Nonempty_iff t).mp ne
+             simp only [starNFA_δ]
+             have ss : t.q₀ ⊆ starNFA_δ t q' a := by simp only [starNFA_δ]
+                                                     split
+                                                     · apply Finset.subset_union_right
+                                                     · rw [Finset.inter_comm] at ne'
+                                                       trivial
+             apply Finset.instIsTransFinsetSubsetInstHasSubsetFinset.trans
+             · exact ss
+             · exact this
+
+
+theorem starNFA_accepts_append (a₁ : nfa_accepts (starNFA t) w₁) (a₂ : nfa_accepts (starNFA t) w₂) : nfa_accepts (starNFA t) (w₁++w₂) := by
+  have := starNFA_accepts_start_subset t a₁
+  simp only [nfa_accepts,δ_star]
+  rw [←δ_star'_append_eq]
+  simp only [nfa_accepts,δ_star,Finset.Nonempty] at a₂
+  have : δ_star' (starNFA t) (starNFA t).q₀ w₂ ⊆ δ_star' (starNFA t) (δ_star' (starNFA t) (starNFA t).q₀ w₁) w₂ := by
+    apply subset_δ_star'_subset
+    exact this
+  apply Exists.elim a₂
+  intro q qin
+  simp only [Finset.Nonempty]
+  exists q
+  rw [Finset.mem_inter] at qin
+  apply Finset.mem_inter.mpr
+  apply And.intro
+  · apply Finset.mem_of_subset
+    · apply this
+    · exact qin.1
+  · exact qin.2
+
+instance instDecidableExWNeNil : Decidable (∃ a, a ∈ nfaLang t ∧ a ≠ []) := by
+  have : Decidable (∃ w, DFA.dfa_accepts (nfa_to_dfa t) w ∧ w ≠ []) := by infer_instance
+  match this with
+  | isTrue h => apply Decidable.isTrue
+                simp only [nfaLang]
+                apply Exists.elim h
+                intro w h
+                rw [←nfa_to_dfa_eq] at h
+                exists w
+  | isFalse h => apply Decidable.isFalse
+                 intro ex
+                 simp only [nfaLang] at ex
+                 apply Exists.elim ex
+                 intro w hin
+                 apply h
+                 exists w
+                 rw [←nfa_to_dfa_eq]
+                 apply hin
+
+lemma nfa_only_nil_star_only_nil : (¬∃ a, a ∈ nfaLang t ∧ a ≠ []) → (nfaLang t = ∅ ∨ nfaLang t = {[]}) := by
+  intro nex
+  cases Decidable.em (Finset.Nonempty (t.q₀ ∩ t.fs)) with
+  | inl h => apply Or.inr
+             simp only [nfaLang,nfa_accepts]
+             rw [Set.eq_singleton_iff_nonempty_unique_mem]
+             apply And.intro
+             · apply Set.nonempty_def.mpr
+               exists []
+             · intro w h
+               rw [not_exists] at nex
+               have := nex w
+               rw [not_and] at this
+               simp only [nfaLang,nfa_accepts] at this
+               rw [Decidable.not_not] at this
+               exact this h
+  | inr h => apply Or.inl
+             simp only [nfaLang,nfa_accepts]
+             rw [Set.eq_empty_iff_forall_not_mem]
+             intro w win
+             rw [not_exists] at nex
+             have := nex w
+             rw [Decidable.not_and] at this
+             apply Or.elim this
+             · intro nin
+               contradiction
+             · intro neq
+               rw [Decidable.not_not] at neq
+               apply h
+               rw [Set.mem_def] at win
+               rw [neq] at win
+               simp only [δ_star,δ_star'] at win
+               exact win
+
+lemma δ_step_star_eq (q : Finset qs): ¬Finset.Nonempty (δ_step t q e ∩ t.fs) → δ_step (starNFA t) q e = δ_step t q e := by
+  intro ne
+  simp only [starNFA,starNFA_δ,δ_step]
+  rw [Finset.eq_iff_fa_mem]
+  intro e'
+  apply Iff.intro
+  · intro ein
+    rw [Finset.mem_biUnion] at ein
+    rw [Finset.mem_biUnion]
+    apply Exists.elim ein
+    intro a ain
+    split at ain
+    · have : False := by apply ne
+                         simp only [δ_step,Finset.biUnion_inter,Finset.Nonempty]
+                         have : Finset.Nonempty (NFA.δ t a e ∩ t.fs) := by assumption
+                         rw [Finset.Nonempty] at this
+                         apply Exists.elim this
+                         intro x xin
+                         exists x
+                         rw [Finset.mem_biUnion]
+                         exists a
+                         exact ⟨ain.1,xin⟩
+      contradiction
+    · exists a
+  · intro ein
+    rw [Finset.mem_biUnion]
+    rw [Finset.mem_biUnion] at ein
+    apply Exists.elim ein
+    intro a ain
+    exists a
+    apply And.intro
+    · exact ain.1
+    · split
+      · exact Finset.mem_union_left _ ain.2
+      · exact ain.2
+
+
+theorem starNFA_split_state : (q : Finset qs) → Finset.Nonempty (δ_star' (starNFA t) q w ∩ (starNFA t).fs) →
+  (Finset.Nonempty (δ_star' t q w ∩ t.fs) ∨ ∃ a b, a ≠ [] ∧ a++b=w ∧ Finset.Nonempty (δ_star' t q a ∩ t.fs) ∧ b ∈ nfaLang (starNFA t)) := by
+  induction w with
+  | nil=> simp only [nfaLang,nfa_accepts,δ_star,δ_star',δ_step]
+          intro h
+          apply Or.inl
+  | cons e es s => intro q acc
+                   simp only [nfaLang,Set.mem_def,nfa_accepts,δ_star] at acc
+                   simp only [nfaLang,Set.mem_def,nfa_accepts,δ_star]
+                   cases Decidable.em (Finset.Nonempty (δ_step t q e ∩ t.fs)) with
+                   | inl h => have eq : δ_star' (starNFA t) q [e] = δ_star' (starNFA t) (δ_star' t q [e] ∪ t.q₀) [] := δ_star'_union_prefinal t q e h
+                              simp only [δ_star'] at eq
+                              simp only [δ_star']
+                              simp only [δ_star'] at acc
+                              have : (starNFA t).q₀ = t.q₀ := by simp [starNFA]
+                              rw [eq] at acc
+                              rw [δ_star'_union] at acc
+                              simp only [Finset.Nonempty] at acc
+                              apply Exists.elim acc
+                              intro x xin
+                              rw [Finset.mem_inter,Finset.mem_union] at xin
+                              apply Or.elim xin.1
+                              · intro xins
+                                have s' := s (δ_step t q e)
+                                have : Finset.Nonempty (δ_star' (starNFA t) (δ_step t q e) es ∩ (starNFA t).fs) := by
+                                  rw [Finset.Nonempty]
+                                  exists x
+                                  rw [Finset.mem_inter]
+                                  exact ⟨xins,xin.2⟩
+                                have := s' this
+                                apply Or.elim this
+                                · intro ne
+                                  apply Or.inl
+                                  exact ne
+                                · intro ex
+                                  apply Exists.elim ex
+                                  intro a ex
+                                  apply Exists.elim ex
+                                  intro b bin
+                                  apply Or.inr
+                                  exists e::a
+                                  exists b
+                                  simp
+                                  use bin.2.1
+                                  apply And.intro
+                                  · exact bin.2.2.1
+                                  · apply bin.2.2.2
+                              · intro xins
+                                apply Or.inr
+                                exists [e]
+                                exists es
+                                simp
+                                apply And.intro
+                                · apply h
+                                · simp only [Finset.Nonempty]
+                                  exists x
+                                  rw [Finset.mem_inter]
+                                  exact ⟨xins,xin.2⟩
+                   | inr h => simp only [δ_star'] at acc
+                              have := s ((δ_step (starNFA t) q e)) acc
+                              apply Or.elim this
+                              · intro e'
+                                apply Or.inl
+                                simp only [δ_star']
+                                rw [δ_step_star_eq] at e'
+                                exact e'
+                                exact h
+                              · intro ex
+                                apply Exists.elim ex
+                                intro a ex
+                                apply Exists.elim ex
+                                intro b bin
+                                apply Or.inr
+                                exists e::a
+                                exists b
+                                simp
+                                use bin.2.1
+                                apply And.intro
+                                · rw [δ_step_star_eq] at bin
+                                  simp only [δ_step] at bin
+                                  exact bin.2.2.1
+                                  exact h
+                                · simp only [nfaLang,nfa_accepts,Set.mem_def] at bin
+                                  exact bin.2.2.2
+
+
+theorem starNfa_split : w ∈ nfaLang (starNFA t) → (w ∈ nfaLang t ∨ ∃ a b, a ≠ [] ∧ a++b=w ∧ a ∈ nfaLang t ∧ b ∈ nfaLang (starNFA t)) := by
+  simp only [nfaLang,nfa_accepts]
+  apply starNFA_split_state
+
+
+theorem no_accept_nfa_starNFA_eq : (¬∃ e es, Finset.Nonempty (δ_star t (e::es) ∩ t.fs)) → ∀ w, (δ_star (starNFA t) w) = δ_star t w := by
+  intro h' w
+  have nex2 : ¬∃ e es, Finset.Nonempty (δ_star t (List.concat es e) ∩ t.fs) := by
+    intro ex
+    apply h'
+    apply Exists.elim ex
+    intro e ex
+    apply Exists.elim ex
+    intro es h
+    have : ∃ b L, List.concat es e = b :: L := List.exists_cons_of_ne_nil (by simp)
+    apply Exists.elim this
+    intro b ex
+    apply Exists.elim ex
+    intro L h
+    exists b
+    exists L
+    rw [←h]
+    trivial
+  have eqδ : ∀ t : (NFA σs qs),∀ w, δ_star' t t.q₀ w = δ_star t w := by
+    intro t w
+    simp only [δ_star]
+  simp only [starNFA,starNFA_δ]
+  induction w using List.reverseRecOn with
+  | H0 => simp
+  | H1 es e s => simp only [δ_star,←δ_star'_append_eq]
+                 simp only [δ_star',δ_step]
+                 rw [eqδ,s,Finset.eq_iff_fa_mem]
+                 intro e'
+                 rw [Finset.mem_biUnion]
+                 apply Iff.intro
+                 · intro ein'
+                   apply Exists.elim ein'
+                   intro q qin
+                   rw [not_exists] at nex2
+                   have := nex2 e
+                   rw [not_exists] at this
+                   have not := this es
+                   rw [List.concat_eq_append] at not
+                   simp only [δ_star] at not
+                   rw [←δ_star'_append_eq] at not
+                   simp only [δ_star'] at not
+                   split at qin
+                   · have : False := by
+                            apply not
+                            have : Finset.Nonempty (NFA.δ t q e ∩ t.fs) := by assumption
+                            rw [Finset.Nonempty] at this
+                            apply Exists.elim this
+                            intro q' qin'
+                            simp only [Finset.Nonempty,δ_step]
+                            rw [Finset.biUnion_inter]
+                            exists q'
+                            rw [Finset.mem_biUnion]
+                            exists q
+                            use qin.1
+                            exact qin'
+                     trivial
+                   · rw [Finset.mem_biUnion]
+                     exists q
+                 · intro ein
+                   rw [Finset.mem_biUnion] at ein
+                   apply Exists.elim ein
+                   intro e ein
+                   exists e
+                   use ein.1
+                   split
+                   · apply Finset.mem_union_left
+                     exact ein.2
+                   · exact ein.2
+
+theorem starNFA_accepts_plusLang : w ∈ nfaLang (starNFA t) ↔ w ∈ Regex.plusLang (nfaLang t) := by
+  simp only [nfaLang]
+  apply Iff.intro
+  · intro win
+    rw [Set.mem_def] at win
+    rw [Set.mem_def]
+    have : w ∈ nfaLang t ∨ ∃ a b, a ≠ [] ∧ a++b=w ∧ a ∈ nfaLang t ∧ b ∈ nfaLang (starNFA t) := starNfa_split t win
+    apply Or.elim this
+    · intro h
+      apply Regex.plusLang.empty
+      apply h
+    · intro h
+      apply Exists.elim h
+      intro a ex
+      apply Exists.elim ex
+      intro b h
+      rw [←h.2.1]
+      have : b.length < w.length := by rw [←h.2.1] -- make clear that the program terminates
+                                       simp only [List.length_append,lt_add_iff_pos_left]
+                                       apply List.length_pos_iff_ne_nil.mpr
+                                       exact h.1
+      apply Regex.plusLang.extend
+      · exact h.2.2.1
+      · apply starNFA_accepts_plusLang.mp -- b is always smaller, so must terminate
+        exact h.2.2.2
+  · intro h
+    induction h with
+    | empty h hin => apply nfa_accepts_starNFA t hin
+    | extend a b h _ s => apply starNFA_accepts_append t (nfa_accepts_starNFA t h) s
+
+termination_by starNFA_accepts_plusLang => w.length
